Route to search implementations from Regex

regex/Regex/Regex/Basic.lean
@@ -3,13 +3,28 @@ import Regex.NFA
 import Regex.VM
 import Regex.Backtracker
 
+open String (Pos Iterator)
+
 structure Regex where
   nfa : Regex.NFA
   wf : nfa.WellFormed
   maxTag : Nat := nfa.maxTag
+  useBacktracker : Bool := false
 deriving Repr
 
 namespace Regex
+
+def captureNextBuf (self : Regex) (bufferSize : Nat) (it : Iterator) : Option (Buffer bufferSize) :=
+  if self.useBacktracker then
+    Backtracker.captureNextBuf self.nfa self.wf bufferSize it
+  else
+    VM.captureNextBuf self.nfa self.wf bufferSize it
+
+def searchNext (self : Regex) (it : Iterator) : Option (Pos × Pos) := do
+  if self.useBacktracker then
+    Backtracker.searchNext self.nfa self.wf it
+  else
+    VM.searchNext self.nfa self.wf it
 
 def parse (s : String) : Except Regex.Syntax.Parser.Error Regex := do
   let expr ← Regex.Syntax.Parser.parse s
