correctness/RegexCorrectness/Regex/Utilities.lean
@@ -11,31 +11,31 @@ namespace Regex
 variable {re : Regex} {haystack : String}
 
 theorem captures_of_find_some {positions} (h : re.find haystack = .some positions)
-  (s : re.IsSearchRegex) :
+  (s : re.IsSearchRegex) (bt : ¬re.useBacktracker) :
   Matches.Spec s haystack positions := by
   simp [Regex.find] at h
   have ⟨_, h⟩ := h
   have v := Captures.valid_captures haystack s
-  exact (Matches.captures_of_next?_some h v).2
+  exact (Matches.captures_of_next?_some h v bt).2
 
 theorem captures_of_mem_findAll.go {m : Matches} {accum : Array (Pos × Pos)}
-  (v : m.Valid) (inv : ∀ positions ∈ accum, Matches.Spec v.1 m.haystack positions) :
+  (v : m.Valid) (bt : ¬m.regex.useBacktracker) (inv : ∀ positions ∈ accum, Matches.Spec v.1 m.haystack positions) :
   ∀ positions ∈ findAll.go m accum, Matches.Spec v.1 m.haystack positions := by
   induction m, accum using findAll.go.induct with
   | case1 m accum positions m' next_some? ih =>
     -- next match is found
     rw [findAll.go, next_some?]
     simp
-    have regex_eq := Matches.regex_eq_of_next?_some next_some?
-    have haystack_eq := Matches.haystack_eq_of_next?_some next_some?
+    have regex_eq := Matches.regex_eq_of_next?_some next_some? bt
+    have haystack_eq := Matches.haystack_eq_of_next?_some next_some? bt
     simp [regex_eq, haystack_eq] at ih
 
-    have ⟨v', spec⟩ := Matches.captures_of_next?_some next_some? v
+    have ⟨v', spec⟩ := Matches.captures_of_next?_some next_some? v bt
     have inv' (p₁ p₂ : Pos) (mem : (p₁, p₂) ∈ accum ∨ (p₁, p₂) = positions) : Matches.Spec v.1 m.haystack (p₁, p₂) := by
       cases mem with
       | inl mem => exact inv (p₁, p₂) mem
       | inr eq => exact eq ▸ spec
-    exact ih v' inv'
+    exact ih v' (by simp [bt]) inv'
   | case2 m accum next_none? =>
     -- next match is not found
     rw [findAll.go, next_none?]
@@ -43,38 +43,38 @@ theorem captures_of_mem_findAll.go {m : Matches} {accum : Array (Pos × Pos)}
     exact inv
 
 theorem captures_of_mem_findAll {positions} (mem : positions ∈ re.findAll haystack)
-  (s : re.IsSearchRegex) :
+  (s : re.IsSearchRegex) (bt : ¬re.useBacktracker) :
   Matches.Spec s haystack positions := by
   simp [Regex.findAll] at mem
   have v := Matches.vaild_matches haystack s
-  exact captures_of_mem_findAll.go v (by simp) positions mem
+  exact captures_of_mem_findAll.go v bt (by simp) positions mem
 
 theorem captures_of_capture_some {captured} (h : re.capture haystack = .some captured)
-  (s : re.IsSearchRegex) :
+  (s : re.IsSearchRegex) (bt : ¬re.useBacktracker) :
   captured.Spec s haystack := by
   simp [Regex.capture] at h
   have ⟨_, h⟩ := h
   have v := Captures.valid_captures haystack s
-  exact (Captures.captures_of_next?_some h v).2
+  exact (Captures.captures_of_next?_some h v bt).2
 
 theorem captures_of_mem_captureAll.go {captures : Captures} {accum : Array CapturedGroups}
-  (v : captures.Valid) (inv : ∀ captured ∈ accum, captured.Spec v.1 captures.haystack) :
+  (v : captures.Valid) (bt : ¬captures.regex.useBacktracker) (inv : ∀ captured ∈ accum, captured.Spec v.1 captures.haystack) :
   ∀ captured ∈ captureAll.go captures accum, captured.Spec v.1 captures.haystack := by
   induction captures, accum using captureAll.go.induct with
   | case1 captures accum groups captures' next?_some ih =>
     -- next capture is found
     rw [captureAll.go, next?_some]
     simp
-    have regex_eq := Captures.regex_eq_of_next?_some next?_some
-    have haystack_eq := Captures.haystack_eq_of_next?_some next?_some
+    have regex_eq := Captures.regex_eq_of_next?_some next?_some bt
+    have haystack_eq := Captures.haystack_eq_of_next?_some next?_some bt
     simp [regex_eq, haystack_eq] at ih
 
-    have ⟨v', spec⟩ := Captures.captures_of_next?_some next?_some v
+    have ⟨v', spec⟩ := Captures.captures_of_next?_some next?_some v bt
     have inv' (captured : CapturedGroups) (mem : captured ∈ accum ∨ captured = groups) : captured.Spec v.1 captures.haystack := by
       cases mem with
       | inl mem => exact inv captured mem
       | inr eq => exact eq ▸ spec
-    exact ih v' inv'
+    exact ih v' (by simp [bt]) inv'
   | case2 captures accum next?_none =>
     -- next capture is not found
     rw [captureAll.go, next?_none]
@@ -82,10 +82,10 @@ theorem captures_of_mem_captureAll.go {captures : Captures} {accum : Array Captu
     exact inv
 
 theorem captures_of_mem_captureAll {captured} (mem : captured ∈ re.captureAll haystack)
-  (s : re.IsSearchRegex) :
+  (s : re.IsSearchRegex) (bt : ¬re.useBacktracker) :
   captured.Spec s haystack := by
   simp [Regex.captureAll] at mem
   have v := Captures.valid_captures haystack s
-  exact captures_of_mem_captureAll.go v (by simp) captured mem
+  exact captures_of_mem_captureAll.go v bt (by simp) captured mem
 
 end Regex
